semantics/semanticsScript.sml
@@ -15,7 +15,6 @@ parse toks =
 
 val _ = Datatype`
   state = <| (* Type system state *)
-            next_comp_unit : num;
             tenv : type_env;
             (* Semantics state *)
             sem_st : 'ffi semanticPrimitives$state;
@@ -25,7 +24,7 @@ val _ = hide "state";
 
 val can_type_prog_def = Define `
 can_type_prog state prog ⇔
-  ∃tdecs' new_tenv. type_ds T state.next_comp_unit state.tenv prog tdecs' new_tenv`;
+  ∃tdecs' new_tenv. type_ds T state.tenv prog tdecs' new_tenv`;
 
 val evaluate_prog_with_clock_def = Define`
   evaluate_prog_with_clock st env k prog =
